src/lowparse/LowParse.SLow.Base.fst
@@ -287,7 +287,7 @@ let parse32_total
 = ()
   
 inline_for_extraction
-let u32_max : (y: U32.t { forall (x: U32.t) . U32.v x <= U32.v y } ) =
+let u32_max : (y: U32.t { forall (x: U32.t) . {:pattern (U32.v x)} U32.v x <= U32.v y } ) =
   4294967295ul
 
 inline_for_extraction
